add smaller ipoptions proofs

deps/poulet4/lib/P4automata/Benchmarks/IPOptions.v
@@ -18,7 +18,7 @@ Ltac prep_equiv :=
 Obligation Tactic := prep_equiv.
 
 
-Module IPOptionsRef.
+Module IPOptionsRef10.
   Inductive state :=
   | Parse0
   | Parse1
@@ -1623,5 +1623,1119 @@ Module IPOptionsRef.
     {| t_states := states |}.
   Solve Obligations with (destruct s; cbv; Lia.lia).
 
-End IPOptionsRef.
+End IPOptionsRef10.
 
+
+
+Module IPOptionsRef5.
+  Inductive state :=
+  | Parse0
+  | Parse1
+  | Parse2
+  | Parse3
+  | Parse4
+
+  | Parse01
+  | Parse11
+  | Parse21
+  | Parse31
+  | Parse41
+  
+  | Parse02
+  | Parse12
+  | Parse22
+  | Parse32
+  | Parse42
+
+  | Parse03
+  | Parse13
+  | Parse23
+  | Parse33
+  | Parse43
+
+  | Parse04
+  | Parse14
+  | Parse24
+  | Parse34
+  | Parse44
+
+  | Parse05
+  | Parse15
+  | Parse25
+  | Parse35
+  | Parse45
+
+  | Parse06
+  | Parse16
+  | Parse26
+  | Parse36
+  | Parse46
+
+  | Parse07
+  | Parse17
+  | Parse27
+  | Parse37
+  | Parse47
+
+  | Parse08
+  | Parse18
+  | Parse28
+  | Parse38
+  | Parse48.
+
+  Scheme Equality for state.
+
+  Global Instance state_eqdec: EquivDec.EqDec state eq := state_eq_dec.
+  Global Program Instance state_finite: @Finite state _ state_eq_dec :=
+    {| enum := [ Parse0 ; Parse1 ; Parse2 ; Parse3 ; Parse4
+    ; Parse01 ; Parse11 ; Parse21 ; Parse31 ; Parse41
+      ; Parse02 ; Parse12 ; Parse22 ; Parse32 ; Parse42
+    ; Parse03 ; Parse13 ; Parse23 ; Parse33 ; Parse43
+    ; Parse04 ; Parse14 ; Parse24 ; Parse34 ; Parse44
+    ; Parse05 ; Parse15 ; Parse25 ; Parse35 ; Parse45
+    ; Parse06 ; Parse16 ; Parse26 ; Parse36 ; Parse46
+    ; Parse07 ; Parse17 ; Parse27 ; Parse37 ; Parse47
+    ; Parse08 ; Parse18 ; Parse28 ; Parse38 ; Parse48 ]; |}.
+  Next Obligation.
+    repeat constructor;
+      repeat match goal with
+             | H: List.In _ [] |- _ => apply List.in_nil in H; exfalso; exact H
+             | |- ~ List.In _ [] => apply List.in_nil
+             | |- ~ List.In _ (_ :: _) => unfold not; intros
+             | H: List.In _ (_::_) |- _ => inversion H; clear H
+             | _ => discriminate
+             end.
+  Qed.
+  Next Obligation.
+    destruct x; intuition congruence.
+  Qed.
+
+  Inductive header : nat -> Type :=
+  | Scratch8 : header 8
+  | Scratch16 : header 16
+  | Scratch24 : header 24
+  | Scratch32 : header 32
+  | Scratch40 : header 40
+  | Scratch48 : header 48
+  | Scratch56 : header 56
+  | T0 : header 8
+  | L0 : header 8
+  | V0 : header 64
+  | T1 : header 8
+  | L1 : header 8
+  | V1 : header 64
+  | T2 : header 8
+  | L2 : header 8
+  | V2 : header 64
+  | T3 : header 8
+  | L3 : header 8
+  | V3 : header 64
+  | T4 : header 8
+  | L4 : header 8
+  | V4 : header 64.
+
+  Derive Signature for header.
+
+  Definition h8_eq_dec (x y: header 8) : {x = y} + {x <> y}.
+    refine (
+    match x with 
+    | Scratch8 =>
+      match y with
+      | Scratch8  => left eq_refl
+      | T0 => right _
+      | L0 => right _
+      | T1 => right _
+      | L1 => right _
+      | T2 => right _
+      | L2 => right _
+      | T3 => right _
+      | L3 => right _
+      | T4 => right _
+      | L4 => right _
+      end
+    | T0 =>
+      match y with
+      | Scratch8  => right _
+      | T0 => left eq_refl
+      | L0 => right _
+      | T1 => right _
+      | L1 => right _
+      | T2 => right _
+      | L2 => right _
+      | T3 => right _
+      | L3 => right _
+      | T4 => right _
+      | L4 => right _
+      end
+      
+    | L0 =>
+      match y with
+      | Scratch8  => right _
+      | T0 => right _
+      | L0 => left eq_refl
+      | T1 => right _
+      | L1 => right _
+      | T2 => right _
+      | L2 => right _
+      | T3 => right _
+      | L3 => right _
+      | T4 => right _
+      | L4 => right _
+      end
+      
+    | T1 =>
+      match y with
+      | Scratch8  => right _
+      | T0 => right _
+      | L0 => right _
+      | T1 => left eq_refl
+      | L1 => right _
+      | T2 => right _
+      | L2 => right _
+      | T3 => right _
+      | L3 => right _
+      | T4 => right _
+      | L4 => right _
+      end
+      
+    | L1 =>
+      match y with
+      | Scratch8  => right _
+      | T0 => right _
+      | L0 => right _
+      | T1 => right _
+      | L1 => left eq_refl
+      | T2 => right _
+      | L2 => right _
+      | T3 => right _
+      | L3 => right _
+      | T4 => right _
+      | L4 => right _
+      end
+      
+    | T2 =>
+      match y with
+      | Scratch8  => right _
+      | T0 => right _
+      | L0 => right _
+      | T1 => right _
+      | L1 => right _
+      | T2 => left eq_refl
+      | L2 => right _
+      | T3 => right _
+      | L3 => right _
+      | T4 => right _
+      | L4 => right _
+      end
+      
+    | L2 =>
+      match y with
+      | Scratch8  => right _
+      | T0 => right _
+      | L0 => right _
+      | T1 => right _
+      | L1 => right _
+      | T2 => right _
+      | L2 => left eq_refl
+      | T3 => right _
+      | L3 => right _
+      | T4 => right _
+      | L4 => right _
+      end
+      
+    | T3 =>
+      match y with
+      | Scratch8  => right _
+      | T0 => right _
+      | L0 => right _
+      | T1 => right _
+      | L1 => right _
+      | T2 => right _
+      | L2 => right _
+      | T3 => left eq_refl
+      | L3 => right _
+      | T4 => right _
+      | L4 => right _
+      end
+      
+    | L3 =>
+      match y with
+      | Scratch8  => right _
+      | T0 => right _
+      | L0 => right _
+      | T1 => right _
+      | L1 => right _
+      | T2 => right _
+      | L2 => right _
+      | T3 => right _
+      | L3 => left eq_refl
+      | T4 => right _
+      | L4 => right _
+      end
+      
+    | T4 =>
+      match y with
+      | Scratch8  => right _
+      | T0 => right _
+      | L0 => right _
+      | T1 => right _
+      | L1 => right _
+      | T2 => right _
+      | L2 => right _
+      | T3 => right _
+      | L3 => right _
+      | T4 => left eq_refl
+      | L4 => right _
+      end
+      
+    | L4 =>
+      match y with
+      | Scratch8  => right _
+      | T0 => right _
+      | L0 => right _
+      | T1 => right _
+      | L1 => right _
+      | T2 => right _
+      | L2 => right _
+      | T3 => right _
+      | L3 => right _
+      | T4 => right _
+      | L4 => left eq_refl
+      end
+    end
+  ); intros H; inversion H.
+  Defined.
+
+  Definition h16_eq_dec (x y: header 16) : {x = y} + {x <> y} :=
+    match x, y with 
+    | Scratch16, Scratch16 => left eq_refl
+    | _, _ => idProp
+    end.
+  Definition h24_eq_dec (x y: header 24) : {x = y} + {x <> y} :=
+    match x, y with 
+    | Scratch24, Scratch24 => left eq_refl
+    | _, _ => idProp
+    end.
+  Definition h32_eq_dec (x y: header 32) : {x = y} + {x <> y} :=
+    match x, y with 
+    | Scratch32, Scratch32 => left eq_refl
+    | _, _ => idProp
+    end.
+  Definition h40_eq_dec (x y: header 40) : {x = y} + {x <> y} :=
+    match x, y with 
+    | Scratch40, Scratch40 => left eq_refl
+    | _, _ => idProp
+    end.
+  Definition h48_eq_dec (x y: header 48) : {x = y} + {x <> y} :=
+    match x, y with 
+    | Scratch48, Scratch48 => left eq_refl
+    | _, _ => idProp
+    end.
+  Definition h56_eq_dec (x y: header 56) : {x = y} + {x <> y} :=
+    match x, y with 
+    | Scratch56, Scratch56 => left eq_refl
+    | _, _ => idProp
+    end.
+
+  Definition h64_eq_dec (x y: header 64) : {x = y} + {x <> y}.
+    refine (
+    match x with 
+    | V0 =>
+      match y with
+      | V0 => left eq_refl
+      | V1 => right _
+      | V2 => right _
+      | V3 => right _
+      | V4 => right _
+      end
+    | V1 =>
+      match y with
+      | V0 => right _
+      | V1 => left eq_refl
+      | V2 => right _
+      | V3 => right _
+      | V4 => right _
+      end
+    | V2 =>
+      match y with
+      | V0 => right _
+      | V1 => right _
+      | V2 => left eq_refl
+      | V3 => right _
+      | V4 => right _
+      end
+    | V3 =>
+      match y with
+      | V0 => right _
+      | V1 => right _
+      | V2 => right _
+      | V3 => left eq_refl
+      | V4 => right _
+      end
+    | V4 =>
+      match y with
+      | V0 => right _
+      | V1 => right _
+      | V2 => right _
+      | V3 => right _
+      | V4 => left eq_refl
+      end
+    end
+  ); intros H; inversion H.
+  Defined.
+
+  Definition header_eqdec_ (n: nat) (x: header n) (y: header n) : {x = y} + {x <> y}.
+    solve_header_eqdec_ n x y 
+      ((existT (fun n => forall x y: header n, {x = y} + {x <> y}) _ h8_eq_dec) :: 
+        (existT _ _ h16_eq_dec) :: (existT _ _ h24_eq_dec) :: (existT _ _ h32_eq_dec) :: 
+        (existT _ _ h40_eq_dec) :: (existT _ _ h48_eq_dec) :: (existT _ _ h56_eq_dec) ::
+        (existT _ _ h64_eq_dec) :: nil).
+  Defined. 
+
+  Global Instance header_eqdec: forall n, EquivDec.EqDec (header n) eq := header_eqdec_.
+
+  Global Instance header_eqdec': EquivDec.EqDec (Syntax.H' header) eq.
+  Proof.
+    solve_eqdec'.
+  Defined.
+
+  Global Instance header_finite: forall n, @Finite (header n) _ _.
+  Proof.
+    intros n; solve_indexed_finiteness n [8; 16; 24; 32; 40; 48; 56; 64].
+  Qed.
+
+  Global Program Instance header_finite': @Finite {n & header n} _ header_eqdec' :=
+    {| enum :=   [existT _ _ Scratch8 ;
+    existT _ _ Scratch16 ;
+    existT _ _ Scratch24 ;
+    existT _ _ Scratch32 ;
+    existT _ _ Scratch40 ;
+    existT _ _ Scratch48 ;
+    existT _ _ Scratch56 ;
+    existT _ _ T0 ;
+    existT _ _ L0 ;
+    existT _ _ V0 ;
+    existT _ _ T1 ;
+    existT _ _ L1 ;
+    existT _ _ V1 ;
+    existT _ _ T2 ;
+    existT _ _ L2 ;
+    existT _ _ V2 ;
+    existT _ _ T3 ;
+    existT _ _ L3 ;
+    existT _ _ V3 ;
+    existT _ _ T4 ;
+    existT _ _ L4 ;
+    existT _ _ V4 
+    ]; |}.
+  Next Obligation.
+    solve_header_finite.
+  Qed.
+  Next Obligation.
+  dependent destruction X; subst;
+  repeat (
+    match goal with
+    | |- ?L \/ ?R => (now left; trivial) || right
+    end
+  ).
+  Qed.
+
+  Definition states (s: state) :=
+    match s with
+    | Parse0 =>
+      {| st_op := 
+          extract(T0) ;;
+          extract(L0) ;
+         st_trans := transition select (| EHdr T0, EHdr L0 |) {{
+           [| exact #b|0|0|0|0|0|0|0|0, exact #b|0|0|0|0|0|0|0|0 |] ==> accept ;;;
+           [| exact #b|0|0|0|0|0|0|0|1, exact #b|0|0|0|0|0|0|0|0 |] ==> accept ;;;
+           [| *, exact #b|0|0|0|0|0|0|0|1 |] ==> inl Parse01 ;;;
+           [| *, exact #b|0|0|0|0|0|0|1|0 |] ==> inl Parse02 ;;;
+           [| *, exact #b|0|0|0|0|0|0|1|1 |] ==> inl Parse03 ;;;
+           [| *, exact #b|0|0|0|0|0|1|0|0 |] ==> inl Parse04 ;;;
+           [| *, exact #b|0|0|0|0|0|1|0|1 |] ==> inl Parse05 ;;;
+           [| *, exact #b|0|0|0|0|0|1|1|0 |] ==> inl Parse06 ;;;
+           [| *, exact #b|0|0|0|0|0|1|1|1 |] ==> inl Parse07 ;;;
+           [| *, exact #b|0|0|0|0|1|0|0|0 |] ==> inl Parse08 ;;;
+            reject
+         }}
+      |}
+    | Parse01 =>
+      {| st_op := 
+          extract(Scratch8) ;;
+          V0 <- EConcat (m := 56) (EHdr Scratch8) ((EHdr V0)[64--8]) ;
+         st_trans := transition inl Parse1;
+      |}
+    | Parse02 =>
+      {| st_op := 
+          extract(Scratch16) ;;
+          V0 <- EConcat (m := 48) (EHdr Scratch16) ((EHdr V0)[64--16]) ;
+         st_trans := transition inl Parse1;
+      |}
+    | Parse03 =>
+      {| st_op := 
+          extract(Scratch24) ;;
+          V0 <- EConcat (m := 40) (EHdr Scratch24) ((EHdr V0)[64--24]) ;
+         st_trans := transition inl Parse1;
+      |}
+    | Parse04 =>
+      {| st_op := 
+          extract(Scratch32) ;;
+          V0 <- EConcat (m := 32) (EHdr Scratch32) ((EHdr V0)[64--32]) ;
+         st_trans := transition inl Parse1;
+      |}
+    | Parse05 =>
+      {| st_op := 
+          extract(Scratch40) ;;
+          V0 <- EConcat (m := 24) (EHdr Scratch40) ((EHdr V0)[64--40]) ;
+         st_trans := transition inl Parse1;
+      |}
+    | Parse06 =>
+      {| st_op := 
+          extract(Scratch48) ;;
+          V0 <- EConcat (m := 16) (EHdr Scratch48) ((EHdr V0)[64--48]) ;
+         st_trans := transition inl Parse1;
+      |}
+    | Parse07 =>
+      {| st_op := 
+          extract(Scratch56) ;;
+          V0 <- EConcat (m := 8) (EHdr Scratch56) ((EHdr V0)[64--56]) ;
+         st_trans := transition inl Parse1;
+      |}
+    | Parse08 =>
+      {| st_op := 
+          extract(V0) ;
+         st_trans := transition inl Parse1;
+      |}
+
+    | Parse1 =>
+      {| st_op := 
+          extract(T1) ;;
+          extract(L1) ;
+         st_trans := transition select (| EHdr T1, EHdr L1 |) {{
+           [| exact #b|0|0|0|0|0|0|0|0, exact #b|0|0|0|0|0|0|0|0 |] ==> accept ;;;
+           [| exact #b|0|0|0|0|0|0|0|1, exact #b|0|0|0|0|0|0|0|0 |] ==> accept ;;;
+           [| *, exact #b|0|0|0|0|0|0|0|1 |] ==> inl Parse11 ;;;
+           [| *, exact #b|0|0|0|0|0|0|1|0 |] ==> inl Parse12 ;;;
+           [| *, exact #b|0|0|0|0|0|0|1|1 |] ==> inl Parse13 ;;;
+           [| *, exact #b|0|0|0|0|0|1|0|0 |] ==> inl Parse14 ;;;
+           [| *, exact #b|0|0|0|0|0|1|0|1 |] ==> inl Parse15 ;;;
+           [| *, exact #b|0|0|0|0|0|1|1|0 |] ==> inl Parse16 ;;;
+           [| *, exact #b|0|0|0|0|0|1|1|1 |] ==> inl Parse17 ;;;
+           [| *, exact #b|0|0|0|0|1|0|0|0 |] ==> inl Parse18 ;;;
+            reject
+         }}
+      |}
+    | Parse11 =>
+      {| st_op := 
+          extract(Scratch8) ;;
+          V1 <- EConcat (m := 56) (EHdr Scratch8) ((EHdr V1)[64--8]) ;
+         st_trans := transition inl Parse2;
+      |}
+    | Parse12 =>
+      {| st_op := 
+          extract(Scratch16) ;;
+          V1 <- EConcat (m := 48) (EHdr Scratch16) ((EHdr V1)[64--16]) ;
+         st_trans := transition inl Parse2;
+      |}
+    | Parse13 =>
+      {| st_op := 
+          extract(Scratch24) ;;
+          V1 <- EConcat (m := 40) (EHdr Scratch24) ((EHdr V1)[64--24]) ;
+         st_trans := transition inl Parse2;
+      |}
+    | Parse14 =>
+      {| st_op := 
+          extract(Scratch32) ;;
+          V1 <- EConcat (m := 32) (EHdr Scratch32) ((EHdr V1)[64--32]) ;
+         st_trans := transition inl Parse2;
+      |}
+    | Parse15 =>
+      {| st_op := 
+          extract(Scratch40) ;;
+          V1 <- EConcat (m := 24) (EHdr Scratch40) ((EHdr V1)[64--40]) ;
+         st_trans := transition inl Parse2;
+      |}
+    | Parse16 =>
+      {| st_op := 
+          extract(Scratch48) ;;
+          V1 <- EConcat (m := 16) (EHdr Scratch48) ((EHdr V1)[64--48]) ;
+         st_trans := transition inl Parse2;
+      |}
+    | Parse17 =>
+      {| st_op := 
+          extract(Scratch56) ;;
+          V1 <- EConcat (m := 8) (EHdr Scratch56) ((EHdr V1)[64--56]) ;
+         st_trans := transition inl Parse2;
+      |}
+    | Parse18 =>
+      {| st_op := 
+          extract(V1) ;
+         st_trans := transition inl Parse2;
+      |}
+
+    | Parse2 =>
+      {| st_op := 
+          extract(T2) ;;
+          extract(L2) ;
+         st_trans := transition select (| EHdr T2, EHdr L2 |) {{
+           [| exact #b|0|0|0|0|0|0|0|0, exact #b|0|0|0|0|0|0|0|0 |] ==> accept ;;;
+           [| exact #b|0|0|0|0|0|0|0|1, exact #b|0|0|0|0|0|0|0|0 |] ==> accept ;;;
+           [| *, exact #b|0|0|0|0|0|0|0|1 |] ==> inl Parse21 ;;;
+           [| *, exact #b|0|0|0|0|0|0|1|0 |] ==> inl Parse22 ;;;
+           [| *, exact #b|0|0|0|0|0|0|1|1 |] ==> inl Parse23 ;;;
+           [| *, exact #b|0|0|0|0|0|1|0|0 |] ==> inl Parse24 ;;;
+           [| *, exact #b|0|0|0|0|0|1|0|1 |] ==> inl Parse25 ;;;
+           [| *, exact #b|0|0|0|0|0|1|1|0 |] ==> inl Parse26 ;;;
+           [| *, exact #b|0|0|0|0|0|1|1|1 |] ==> inl Parse27 ;;;
+           [| *, exact #b|0|0|0|0|1|0|0|0 |] ==> inl Parse28 ;;;
+            reject
+         }}
+      |}
+    | Parse21 =>
+      {| st_op := 
+          extract(Scratch8) ;;
+          V1 <- EConcat (m := 56) (EHdr Scratch8) ((EHdr V2)[64--8]) ;
+         st_trans := transition inl Parse3;
+      |}
+    | Parse22 =>
+      {| st_op := 
+          extract(Scratch16) ;;
+          V2 <- EConcat (m := 48) (EHdr Scratch16) ((EHdr V2)[64--16]) ;
+         st_trans := transition inl Parse3;
+      |}
+    | Parse23 =>
+      {| st_op := 
+          extract(Scratch24) ;;
+          V2 <- EConcat (m := 40) (EHdr Scratch24) ((EHdr V2)[64--24]) ;
+         st_trans := transition inl Parse3;
+      |}
+    | Parse24 =>
+      {| st_op := 
+          extract(Scratch32) ;;
+          V2 <- EConcat (m := 32) (EHdr Scratch32) ((EHdr V2)[64--32]) ;
+         st_trans := transition inl Parse3;
+      |}
+    | Parse25 =>
+      {| st_op := 
+          extract(Scratch40) ;;
+          V2 <- EConcat (m := 24) (EHdr Scratch40) ((EHdr V2)[64--40]) ;
+         st_trans := transition inl Parse3;
+      |}
+    | Parse26 =>
+      {| st_op := 
+          extract(Scratch48) ;;
+          V2 <- EConcat (m := 16) (EHdr Scratch48) ((EHdr V2)[64--48]) ;
+         st_trans := transition inl Parse3;
+      |}
+    | Parse27 =>
+      {| st_op := 
+          extract(Scratch56) ;;
+          V2 <- EConcat (m := 8) (EHdr Scratch56) ((EHdr V2)[64--56]) ;
+         st_trans := transition inl Parse3;
+      |}
+    | Parse28 =>
+      {| st_op := 
+          extract(V2) ;
+         st_trans := transition inl Parse3;
+      |}
+
+    | Parse3 =>
+      {| st_op := 
+          extract(T3) ;;
+          extract(L3) ;
+         st_trans := transition select (| EHdr T3, EHdr L3 |) {{
+           [| exact #b|0|0|0|0|0|0|0|0, exact #b|0|0|0|0|0|0|0|0 |] ==> accept ;;;
+           [| exact #b|0|0|0|0|0|0|0|1, exact #b|0|0|0|0|0|0|0|0 |] ==> accept ;;;
+           [| *, exact #b|0|0|0|0|0|0|0|1 |] ==> inl Parse31 ;;;
+           [| *, exact #b|0|0|0|0|0|0|1|0 |] ==> inl Parse32 ;;;
+           [| *, exact #b|0|0|0|0|0|0|1|1 |] ==> inl Parse33 ;;;
+           [| *, exact #b|0|0|0|0|0|1|0|0 |] ==> inl Parse34 ;;;
+           [| *, exact #b|0|0|0|0|0|1|0|1 |] ==> inl Parse35 ;;;
+           [| *, exact #b|0|0|0|0|0|1|1|0 |] ==> inl Parse36 ;;;
+           [| *, exact #b|0|0|0|0|0|1|1|1 |] ==> inl Parse37 ;;;
+           [| *, exact #b|0|0|0|0|1|0|0|0 |] ==> inl Parse38 ;;;
+            reject
+         }}
+      |}
+    | Parse31 =>
+      {| st_op := 
+          extract(Scratch8) ;;
+          V3 <- EConcat (m := 56) (EHdr Scratch8) ((EHdr V3)[64--8]) ;
+         st_trans := transition inl Parse4;
+      |}
+    | Parse32 =>
+      {| st_op := 
+          extract(Scratch16) ;;
+          V3 <- EConcat (m := 48) (EHdr Scratch16) ((EHdr V3)[64--16]) ;
+         st_trans := transition inl Parse4;
+      |}
+    | Parse33 =>
+      {| st_op := 
+          extract(Scratch24) ;;
+          V3 <- EConcat (m := 40) (EHdr Scratch24) ((EHdr V3)[64--24]) ;
+         st_trans := transition inl Parse4;
+      |}
+    | Parse34 =>
+      {| st_op := 
+          extract(Scratch32) ;;
+          V3 <- EConcat (m := 32) (EHdr Scratch32) ((EHdr V3)[64--32]) ;
+         st_trans := transition inl Parse4;
+      |}
+    | Parse35 =>
+      {| st_op := 
+          extract(Scratch40) ;;
+          V3 <- EConcat (m := 24) (EHdr Scratch40) ((EHdr V3)[64--40]) ;
+         st_trans := transition inl Parse4;
+      |}
+    | Parse36 =>
+      {| st_op := 
+          extract(Scratch48) ;;
+          V3 <- EConcat (m := 16) (EHdr Scratch48) ((EHdr V3)[64--48]) ;
+         st_trans := transition inl Parse4;
+      |}
+    | Parse37 =>
+      {| st_op := 
+          extract(Scratch56) ;;
+          V3 <- EConcat (m := 8) (EHdr Scratch56) ((EHdr V3)[64--56]) ;
+         st_trans := transition inl Parse4;
+      |}
+    | Parse38 =>
+      {| st_op := 
+          extract(V3) ;
+         st_trans := transition inl Parse4;
+      |}
+      
+    | Parse4 =>
+      {| st_op := 
+          extract(T4) ;;
+          extract(L4) ;
+         st_trans := transition select (| EHdr T4, EHdr L4 |) {{
+           [| exact #b|0|0|0|0|0|0|0|0, exact #b|0|0|0|0|0|0|0|0 |] ==> accept ;;;
+           [| exact #b|0|0|0|0|0|0|0|1, exact #b|0|0|0|0|0|0|0|0 |] ==> accept ;;;
+           [| *, exact #b|0|0|0|0|0|0|0|1 |] ==> inl Parse41 ;;;
+           [| *, exact #b|0|0|0|0|0|0|1|0 |] ==> inl Parse42 ;;;
+           [| *, exact #b|0|0|0|0|0|0|1|1 |] ==> inl Parse43 ;;;
+           [| *, exact #b|0|0|0|0|0|1|0|0 |] ==> inl Parse44 ;;;
+           [| *, exact #b|0|0|0|0|0|1|0|1 |] ==> inl Parse45 ;;;
+           [| *, exact #b|0|0|0|0|0|1|1|0 |] ==> inl Parse46 ;;;
+           [| *, exact #b|0|0|0|0|0|1|1|1 |] ==> inl Parse47 ;;;
+           [| *, exact #b|0|0|0|0|1|0|0|0 |] ==> inl Parse48 ;;;
+            reject
+         }}
+      |}
+    | Parse41 =>
+      {| st_op := 
+          extract(Scratch8) ;;
+          V4 <- EConcat (m := 56) (EHdr Scratch8) ((EHdr V4)[64--8]) ;
+         st_trans := transition accept;
+      |}
+    | Parse42 =>
+      {| st_op := 
+          extract(Scratch16) ;;
+          V4 <- EConcat (m := 48) (EHdr Scratch16) ((EHdr V4)[64--16]) ;
+         st_trans := transition accept;
+      |}
+    | Parse43 =>
+      {| st_op := 
+          extract(Scratch24) ;;
+          V4 <- EConcat (m := 40) (EHdr Scratch24) ((EHdr V4)[64--24]) ;
+         st_trans := transition accept;
+      |}
+    | Parse44 =>
+      {| st_op := 
+          extract(Scratch32) ;;
+          V4 <- EConcat (m := 32) (EHdr Scratch32) ((EHdr V4)[64--32]) ;
+         st_trans := transition accept;
+      |}
+    | Parse45 =>
+      {| st_op := 
+          extract(Scratch40) ;;
+          V4 <- EConcat (m := 24) (EHdr Scratch40) ((EHdr V4)[64--40]) ;
+         st_trans := transition accept;
+      |}
+    | Parse46 =>
+      {| st_op := 
+          extract(Scratch48) ;;
+          V4 <- EConcat (m := 16) (EHdr Scratch48) ((EHdr V4)[64--48]) ;
+         st_trans := transition accept;
+      |}
+    | Parse47 =>
+      {| st_op := 
+          extract(Scratch56) ;;
+          V4 <- EConcat (m := 8) (EHdr Scratch56) ((EHdr V4)[64--56]) ;
+         st_trans := transition accept;
+      |}
+    | Parse48 =>
+      {| st_op := 
+          extract(V4) ;
+         st_trans := transition accept;
+      |}
+    end.
+
+  Program Definition aut: Syntax.t state header :=
+    {| t_states := states |}.
+  Solve Obligations with (destruct s; cbv; Lia.lia).
+
+End IPOptionsRef5.
+
+
+
+Module IPOptionsRef2.
+  Inductive state :=
+  | Parse0
+  | Parse1
+
+  | Parse01
+  | Parse11
+  
+  | Parse02
+  | Parse12
+
+  | Parse03
+  | Parse13
+
+  | Parse04
+  | Parse14
+
+  | Parse05
+  | Parse15
+
+  | Parse06
+  | Parse16
+
+  | Parse07
+  | Parse17
+
+  | Parse08
+  | Parse18.
+
+  Scheme Equality for state.
+
+  Global Instance state_eqdec: EquivDec.EqDec state eq := state_eq_dec.
+  Global Program Instance state_finite: @Finite state _ state_eq_dec :=
+    {| enum := [  Parse0 ; Parse1
+    ; Parse01 ; Parse11
+      ; Parse02 ; Parse12
+    ; Parse03 ; Parse13
+    ; Parse04 ; Parse14
+    ; Parse05 ; Parse15
+    ; Parse06 ; Parse16
+    ; Parse07 ; Parse17
+    ; Parse08 ; Parse18 ]; |}.
+  Next Obligation.
+    repeat constructor;
+      repeat match goal with
+             | H: List.In _ [] |- _ => apply List.in_nil in H; exfalso; exact H
+             | |- ~ List.In _ [] => apply List.in_nil
+             | |- ~ List.In _ (_ :: _) => unfold not; intros
+             | H: List.In _ (_::_) |- _ => inversion H; clear H
+             | _ => discriminate
+             end.
+  Qed.
+  Next Obligation.
+    destruct x; intuition congruence.
+  Qed.
+
+  Inductive header : nat -> Type :=
+  | Scratch8 : header 8
+  | Scratch16 : header 16
+  | Scratch24 : header 24
+  | Scratch32 : header 32
+  | Scratch40 : header 40
+  | Scratch48 : header 48
+  | Scratch56 : header 56
+  | T0 : header 8
+  | L0 : header 8
+  | V0 : header 64
+  | T1 : header 8
+  | L1 : header 8
+  | V1 : header 64.
+
+  Derive Signature for header.
+
+  Definition h8_eq_dec (x y: header 8) : {x = y} + {x <> y}.
+    refine (
+    match x with 
+    | Scratch8 =>
+      match y with
+      | Scratch8  => left eq_refl
+      | T0 => right _
+      | L0 => right _
+      | T1 => right _
+      | L1 => right _
+      end
+    | T0 =>
+      match y with
+      | Scratch8  => right _
+      | T0 => left eq_refl
+      | L0 => right _
+      | T1 => right _
+      | L1 => right _
+      end
+      
+    | L0 =>
+      match y with
+      | Scratch8  => right _
+      | T0 => right _
+      | L0 => left eq_refl
+      | T1 => right _
+      | L1 => right _
+      end
+      
+    | T1 =>
+      match y with
+      | Scratch8  => right _
+      | T0 => right _
+      | L0 => right _
+      | T1 => left eq_refl
+      | L1 => right _
+      end
+      
+    | L1 =>
+      match y with
+      | Scratch8  => right _
+      | T0 => right _
+      | L0 => right _
+      | T1 => right _
+      | L1 => left eq_refl
+      end
+    end
+  ); intros H; inversion H.
+  Defined.
+
+  Definition h16_eq_dec (x y: header 16) : {x = y} + {x <> y} :=
+    match x, y with 
+    | Scratch16, Scratch16 => left eq_refl
+    | _, _ => idProp
+    end.
+  Definition h24_eq_dec (x y: header 24) : {x = y} + {x <> y} :=
+    match x, y with 
+    | Scratch24, Scratch24 => left eq_refl
+    | _, _ => idProp
+    end.
+  Definition h32_eq_dec (x y: header 32) : {x = y} + {x <> y} :=
+    match x, y with 
+    | Scratch32, Scratch32 => left eq_refl
+    | _, _ => idProp
+    end.
+  Definition h40_eq_dec (x y: header 40) : {x = y} + {x <> y} :=
+    match x, y with 
+    | Scratch40, Scratch40 => left eq_refl
+    | _, _ => idProp
+    end.
+  Definition h48_eq_dec (x y: header 48) : {x = y} + {x <> y} :=
+    match x, y with 
+    | Scratch48, Scratch48 => left eq_refl
+    | _, _ => idProp
+    end.
+  Definition h56_eq_dec (x y: header 56) : {x = y} + {x <> y} :=
+    match x, y with 
+    | Scratch56, Scratch56 => left eq_refl
+    | _, _ => idProp
+    end.
+
+  Definition h64_eq_dec (x y: header 64) : {x = y} + {x <> y}.
+    refine (
+    match x with 
+    | V0 =>
+      match y with
+      | V0 => left eq_refl
+      | V1 => right _
+      end
+    | V1 =>
+      match y with
+      | V0 => right _
+      | V1 => left eq_refl
+      end
+    end
+  ); intros H; inversion H.
+  Defined.
+
+  Definition header_eqdec_ (n: nat) (x: header n) (y: header n) : {x = y} + {x <> y}.
+    solve_header_eqdec_ n x y 
+      ((existT (fun n => forall x y: header n, {x = y} + {x <> y}) _ h8_eq_dec) :: 
+        (existT _ _ h16_eq_dec) :: (existT _ _ h24_eq_dec) :: (existT _ _ h32_eq_dec) :: 
+        (existT _ _ h40_eq_dec) :: (existT _ _ h48_eq_dec) :: (existT _ _ h56_eq_dec) ::
+        (existT _ _ h64_eq_dec) :: nil).
+  Defined. 
+
+  Global Instance header_eqdec: forall n, EquivDec.EqDec (header n) eq := header_eqdec_.
+
+  Global Instance header_eqdec': EquivDec.EqDec (Syntax.H' header) eq.
+  Proof.
+    solve_eqdec'.
+  Defined.
+
+  Global Instance header_finite: forall n, @Finite (header n) _ _.
+  Proof.
+    intros n; solve_indexed_finiteness n [8; 16; 24; 32; 40; 48; 56; 64].
+  Qed.
+
+  Global Program Instance header_finite': @Finite {n & header n} _ header_eqdec' :=
+    {| enum :=   [existT _ _ Scratch8 ;
+    existT _ _ Scratch16 ;
+    existT _ _ Scratch24 ;
+    existT _ _ Scratch32 ;
+    existT _ _ Scratch40 ;
+    existT _ _ Scratch48 ;
+    existT _ _ Scratch56 ;
+    existT _ _ T0 ;
+    existT _ _ L0 ;
+    existT _ _ V0 ;
+    existT _ _ T1 ;
+    existT _ _ L1 ;
+    existT _ _ V1 
+    ]; |}.
+  Next Obligation.
+    solve_header_finite.
+  Qed.
+  Next Obligation.
+  dependent destruction X; subst;
+  repeat (
+    match goal with
+    | |- ?L \/ ?R => (now left; trivial) || right
+    end
+  ).
+  Qed.
+
+  Definition states (s: state) :=
+    match s with
+    | Parse0 =>
+      {| st_op := 
+          extract(T0) ;;
+          extract(L0) ;
+         st_trans := transition select (| EHdr T0, EHdr L0 |) {{
+           [| exact #b|0|0|0|0|0|0|0|0, exact #b|0|0|0|0|0|0|0|0 |] ==> accept ;;;
+           [| exact #b|0|0|0|0|0|0|0|1, exact #b|0|0|0|0|0|0|0|0 |] ==> accept ;;;
+           [| *, exact #b|0|0|0|0|0|0|0|1 |] ==> inl Parse01 ;;;
+           [| *, exact #b|0|0|0|0|0|0|1|0 |] ==> inl Parse02 ;;;
+           [| *, exact #b|0|0|0|0|0|0|1|1 |] ==> inl Parse03 ;;;
+           [| *, exact #b|0|0|0|0|0|1|0|0 |] ==> inl Parse04 ;;;
+           [| *, exact #b|0|0|0|0|0|1|0|1 |] ==> inl Parse05 ;;;
+           [| *, exact #b|0|0|0|0|0|1|1|0 |] ==> inl Parse06 ;;;
+           [| *, exact #b|0|0|0|0|0|1|1|1 |] ==> inl Parse07 ;;;
+           [| *, exact #b|0|0|0|0|1|0|0|0 |] ==> inl Parse08 ;;;
+            reject
+         }}
+      |}
+    | Parse01 =>
+      {| st_op := 
+          extract(Scratch8) ;;
+          V0 <- EConcat (m := 56) (EHdr Scratch8) ((EHdr V0)[64--8]) ;
+         st_trans := transition inl Parse1;
+      |}
+    | Parse02 =>
+      {| st_op := 
+          extract(Scratch16) ;;
+          V0 <- EConcat (m := 48) (EHdr Scratch16) ((EHdr V0)[64--16]) ;
+         st_trans := transition inl Parse1;
+      |}
+    | Parse03 =>
+      {| st_op := 
+          extract(Scratch24) ;;
+          V0 <- EConcat (m := 40) (EHdr Scratch24) ((EHdr V0)[64--24]) ;
+         st_trans := transition inl Parse1;
+      |}
+    | Parse04 =>
+      {| st_op := 
+          extract(Scratch32) ;;
+          V0 <- EConcat (m := 32) (EHdr Scratch32) ((EHdr V0)[64--32]) ;
+         st_trans := transition inl Parse1;
+      |}
+    | Parse05 =>
+      {| st_op := 
+          extract(Scratch40) ;;
+          V0 <- EConcat (m := 24) (EHdr Scratch40) ((EHdr V0)[64--40]) ;
+         st_trans := transition inl Parse1;
+      |}
+    | Parse06 =>
+      {| st_op := 
+          extract(Scratch48) ;;
+          V0 <- EConcat (m := 16) (EHdr Scratch48) ((EHdr V0)[64--48]) ;
+         st_trans := transition inl Parse1;
+      |}
+    | Parse07 =>
+      {| st_op := 
+          extract(Scratch56) ;;
+          V0 <- EConcat (m := 8) (EHdr Scratch56) ((EHdr V0)[64--56]) ;
+         st_trans := transition inl Parse1;
+      |}
+    | Parse08 =>
+      {| st_op := 
+          extract(V0) ;
+         st_trans := transition inl Parse1;
+      |}
+
+    | Parse1 =>
+      {| st_op := 
+          extract(T1) ;;
+          extract(L1) ;
+         st_trans := transition select (| EHdr T1, EHdr L1 |) {{
+           [| exact #b|0|0|0|0|0|0|0|0, exact #b|0|0|0|0|0|0|0|0 |] ==> accept ;;;
+           [| exact #b|0|0|0|0|0|0|0|1, exact #b|0|0|0|0|0|0|0|0 |] ==> accept ;;;
+           [| *, exact #b|0|0|0|0|0|0|0|1 |] ==> inl Parse11 ;;;
+           [| *, exact #b|0|0|0|0|0|0|1|0 |] ==> inl Parse12 ;;;
+           [| *, exact #b|0|0|0|0|0|0|1|1 |] ==> inl Parse13 ;;;
+           [| *, exact #b|0|0|0|0|0|1|0|0 |] ==> inl Parse14 ;;;
+           [| *, exact #b|0|0|0|0|0|1|0|1 |] ==> inl Parse15 ;;;
+           [| *, exact #b|0|0|0|0|0|1|1|0 |] ==> inl Parse16 ;;;
+           [| *, exact #b|0|0|0|0|0|1|1|1 |] ==> inl Parse17 ;;;
+           [| *, exact #b|0|0|0|0|1|0|0|0 |] ==> inl Parse18 ;;;
+            reject
+         }}
+      |}
+    | Parse11 =>
+      {| st_op := 
+          extract(Scratch8) ;;
+          V1 <- EConcat (m := 56) (EHdr Scratch8) ((EHdr V1)[64--8]) ;
+         st_trans := transition accept;
+      |}
+    | Parse12 =>
+      {| st_op := 
+          extract(Scratch16) ;;
+          V1 <- EConcat (m := 48) (EHdr Scratch16) ((EHdr V1)[64--16]) ;
+         st_trans := transition accept;
+      |}
+    | Parse13 =>
+      {| st_op := 
+          extract(Scratch24) ;;
+          V1 <- EConcat (m := 40) (EHdr Scratch24) ((EHdr V1)[64--24]) ;
+         st_trans := transition accept;
+      |}
+    | Parse14 =>
+      {| st_op := 
+          extract(Scratch32) ;;
+          V1 <- EConcat (m := 32) (EHdr Scratch32) ((EHdr V1)[64--32]) ;
+         st_trans := transition accept;
+      |}
+    | Parse15 =>
+      {| st_op := 
+          extract(Scratch40) ;;
+          V1 <- EConcat (m := 24) (EHdr Scratch40) ((EHdr V1)[64--40]) ;
+         st_trans := transition accept;
+      |}
+    | Parse16 =>
+      {| st_op := 
+          extract(Scratch48) ;;
+          V1 <- EConcat (m := 16) (EHdr Scratch48) ((EHdr V1)[64--48]) ;
+         st_trans := transition accept;
+      |}
+    | Parse17 =>
+      {| st_op := 
+          extract(Scratch56) ;;
+          V1 <- EConcat (m := 8) (EHdr Scratch56) ((EHdr V1)[64--56]) ;
+         st_trans := transition accept;
+      |}
+    | Parse18 =>
+      {| st_op := 
+          extract(V1) ;
+         st_trans := transition accept;
+      |}
+    end.
+
+  Program Definition aut: Syntax.t state header :=
+    {| t_states := states |}.
+  Solve Obligations with (destruct s; cbv; Lia.lia).
+
+End IPOptionsRef2.
