deps/poulet4/lib/P4automata/Benchmarks/IPOptionsProof.v
@@ -4,7 +4,7 @@ Require Import Poulet4.P4automata.Benchmarks.IPOptions.
 
 Declare ML Module "mirrorsolve".
 
-Module SelfComparison.
+(* Module SelfComparison.
     
   Notation H := (IPOptionsRef.header + IPOptionsRef.header).
   Notation A := (Sum.sum IPOptionsRef.aut IPOptionsRef.aut).
@@ -92,4 +92,74 @@ Module SelfComparison.
     time "build phase" repeat (time "single step" run_bisim top top' r_states).
     time "close phase" close_bisim top'.
   Time Admitted.
+End SelfComparison. *)
+
+Module SelfComparison.
+    
+  Notation H := (IPOptionsRef2.header + IPOptionsRef2.header).
+  Notation A := (Sum.sum IPOptionsRef2.aut IPOptionsRef2.aut).
+  Notation conf := (P4automaton.configuration (P4A.interp A)).
+  Definition r_states :=
+    Eval vm_compute in (Reachability.reachable_states
+                          A
+                          10
+                          IPOptionsRef2.Parse0
+                          IPOptionsRef2.Parse0).
+
+  Definition top : Relations.rel conf := fun _ _ => True.
+  Definition top' : Relations.rel (state_template A) := fun _ _ => True.
+
+  ClearEnvCtors.
+
+  RegisterEnvCtors
+    (IPOptionsRef5.Scratch8, FirstOrderConfRelSimplified.Bits 8)
+    (  IPOptionsRef5.Scratch16, FirstOrderConfRelSimplified.Bits 16)
+    (  IPOptionsRef5.Scratch24, FirstOrderConfRelSimplified.Bits 24)
+    (  IPOptionsRef5.Scratch32, FirstOrderConfRelSimplified.Bits 32)
+    (  IPOptionsRef5.Scratch40, FirstOrderConfRelSimplified.Bits 40)
+    (  IPOptionsRef5.Scratch48, FirstOrderConfRelSimplified.Bits 48)
+    (  IPOptionsRef5.Scratch56, FirstOrderConfRelSimplified.Bits 56)
+    (  IPOptionsRef5.T0, FirstOrderConfRelSimplified.Bits 8)
+    (  IPOptionsRef5.L0, FirstOrderConfRelSimplified.Bits 8)
+    (  IPOptionsRef5.V0, FirstOrderConfRelSimplified.Bits 64)
+    (  IPOptionsRef5.T1, FirstOrderConfRelSimplified.Bits 8)
+    (  IPOptionsRef5.L1, FirstOrderConfRelSimplified.Bits 8)
+    (  IPOptionsRef5.V1, FirstOrderConfRelSimplified.Bits 64)
+    (  IPOptionsRef5.T2, FirstOrderConfRelSimplified.Bits 8)
+    (  IPOptionsRef5.L2, FirstOrderConfRelSimplified.Bits 8)
+    (  IPOptionsRef5.V2, FirstOrderConfRelSimplified.Bits 64).
+
+  Lemma prebisim_babyip:
+    forall q1 q2,
+      interp_conf_rel' {| cr_st := {|
+                          cs_st1 := {|
+                            st_state := inl (inl (IPOptionsRef2.Parse0));
+                            st_buf_len := 0;
+                          |};
+                          cs_st2 := {|
+                            st_state := inl (inr (IPOptionsRef2.Parse0));
+                            st_buf_len := 0;
+                          |};
+                        |};
+                        cr_ctx := BCEmp;
+                        cr_rel := btrue;
+                    |} q1 q2 ->
+    pre_bisimulation A
+                    (wp r_states)
+                    top
+                    []
+                    (mk_init _ _ _ A 10 IPOptionsRef2.Parse0 IPOptionsRef2.Parse0)
+                    q1 q2.
+  Proof.
+    idtac "running ipoptions ref self-comparison bisimulation".
+
+    intros.
+    set (rel0 := (mk_init _ _ _ A 10 IPOptionsRef2.Parse0 IPOptionsRef2.Parse0)).
+    vm_compute in rel0.
+    subst rel0.
+
+    time "build phase" repeat (time "single step" run_bisim top top' r_states).
+    time "close phase" close_bisim top'.
+  Time Admitted.
 End SelfComparison.
+
